{
  "nbformat": 4,
  "nbformat_minor": 0,
  "metadata": {
    "colab": {
      "provenance": []
    },
    "kernelspec": {
      "name": "python3",
      "display_name": "Python 3"
    },
    "language_info": {
      "name": "python"
    }
  },
  "cells": [
    {
      "cell_type": "markdown",
      "source": [
        "**DISCRETE MATHEMATICS II ASIGNMENT [LECTURE 1]**\n",
        "\n",
        "\n"
      ],
      "metadata": {
        "id": "vPsaXJfFzK6o"
      }
    },
    {
      "cell_type": "markdown",
      "source": [
        "**Name:** Jomar T. Cunado <br>\n",
        "**Program & Year:** BSCS - 1"
      ],
      "metadata": {
        "id": "9Rnolyr5zVZV"
      }
    },
    {
      "cell_type": "markdown",
      "source": [
        "\n",
        "$\\textbf{Assignment}$\n",
        "Instructions:\n",
        "- Use latex.\n",
        "- Write your latex in jupyter notebook.\n",
        "- Push your answer to your github account.\n",
        "- Deadline is 2 weeks before finals.\n",
        "- Fail to submit 2 weeks before finals is an automatic 5.0 for this assignment.\n",
        "- Each problem is 25 points.\n",
        "\n",
        "1. Recall the definition of a rational number, denoted as $\\mathbb{Q}$. Prove that the Euler's number $e = \\Sigma_{k=0}^\\infty \\frac{1}{k!} \\notin \\mathbb{Q}$. A factorial is defined as $k! = (k)(k-1)(k-2)(k-3)..., \\forall k \\in \\mathbb{Z}^+$, note that $0! = 1$. Furthermore, a sum notation $\\Sigma_{k=0}^\\infty k = 0+ 1 + 2 + 3 +....+...$\n",
        "\n",
        "**ANSWER:**\n",
        "\n",
        "Step 1: To prove that Euler's number\n",
        " is irrational, we'll proceed by contradiction.\n",
        "\n",
        "  Assume, for the sake of contradiction, that $e$ is rational. This means that $e$ can be expressed as a fraction $\\frac{p}{q}$ where $p$ and $q$ are integers with no common factors other than 1, and $q \\neq 0$.\n",
        "\n",
        "Step 2: Recall the definition of $e$ as the sum of the infinite series:\n",
        "\n",
        "\n",
        "$ e = \\Sigma_{k=0}^\\infty \\frac{1}{k!}$\n",
        "​\n",
        "\n",
        "Step 3: Consider the partial sums of the series. Let $S_n$ denote the $n$th partial sum:\n",
        "\n",
        "$S_n = \\Sigma_{k=0}^\\infty \\frac{1}{k!}$\n",
        "\n",
        "Step 4: Recognize that $e$ is defined as the limit of these partial sums as $n$ approaches infinity:\n",
        "\n",
        "$e = \\lim_{n \\to \\infty} S_n$\n",
        "\n",
        "Step 5: Since $e$ is rational, $S_n$ must also approach a rational limit as $n$ goes to infinity.\n",
        "\n",
        "Step 6: Notice that each term in the series $\\frac{1}{k!}$ is positive. Therefore, each partial sum $S_n$ is increasing.\n",
        "\n",
        "Step 7: Consider the factorial terms $k!$. For any $k \\geq 1$, we have $k! > k$, which implies $\\frac{1}{k!} < \\frac{1}{k}$.\n",
        "\n",
        "Step 8: Recognize that the series $\\sum_{k=0}^\\infty \\frac{1}{k}$ diverges (known as the harmonic series).\n",
        "\n",
        "Step 9: Since $\\frac{1}{k!} < \\frac{1}{k}$, we can conclude that the series $\\sum_{k=0}^\\infty \\frac{1}{k!}$ converges.\n",
        "\n",
        "Step 10: If $S_n$ converges to a rational number, it must be bounded.\n",
        "\n",
        "Step 11: But the convergence of $\\sum_{k=0}^\\infty \\frac{1}{k!}$ contradicts the unboundedness of the harmonic series.\n",
        "\n",
        "**In Conclusion**, assuming $e$ is rational leads to a contradiction, we conclude that $e$ is not rational, i.e., $e \\notin \\mathbb{Q}$.  \n",
        "\n",
        "\n",
        "<br><br>\n",
        "\n",
        "2. Prove Minkowski's Inequality for sums, $\\forall \\ p>1, (a_k, b_k)>0$:\n",
        "\\begin{gather}\n",
        "\\begin{bmatrix}\n",
        "\\Sigma_{k=1}^n |a_k + b_k|^p\n",
        "\\end{bmatrix}^\\frac{1}{p}\n",
        "\\leq\n",
        "\\begin{bmatrix}\n",
        "\\Sigma_{k=1}^n |a_k|^p\n",
        "\\end{bmatrix}^\\frac{1}{p}\n",
        "+\n",
        "\\begin{bmatrix}\n",
        "\\Sigma_{k=1}^n |b_k|^p\n",
        "\\end{bmatrix}^\\frac{1}{p}\n",
        "\\end{gather}\n",
        "\n",
        "**ANSWER:**\n",
        "\n",
        "Step 1: Laws of Exponents (Power raised to a power):\n",
        "\n",
        "- Let $n = $ any base number, then ${(n^p)}^\\frac{1}{p}=n$\n",
        "- It is known that ${(n^p)}^\\frac{1}{p}=n$ for any base number $n$, which implies that the $p$-th root of $n^p$ is $n$. Applying this to the sums of $|a_k|^p$ and $|b_k|^p$, we have:\n",
        "\n",
        "\\begin{gather}\n",
        "\\Sigma_{k=1}^n |a_k + b_k|\n",
        "\\leq\n",
        "\\Sigma_{k=1}^n |a_k|\n",
        "+\n",
        "\\Sigma_{k=1}^n |b_k|\n",
        "\\end{gather}\n",
        "\n",
        "Step 2: Property of Summation (Addition)\n",
        "\n",
        "\\begin{gather}\n",
        "\\Sigma_{k=1}^n |a_k + b_k|\n",
        "\\leq\n",
        "\\Sigma_{k=1}^n |a_k| + |b_k|\n",
        "\\end{gather}\n",
        "\n",
        "Step 3: Prove by Triangle Inequality\n",
        "\n",
        "- Disregarding the Sigma Notation, we get:\n",
        "\\begin{gather}\n",
        "|a_k + b_k|\n",
        "\\leq\n",
        "|a_k| + b_k|\n",
        "\\end{gather}\n",
        "\n",
        "- Since, $(a_k, b_k) > 0$, then $(a + b) = a + b$, and $|a| = a_k$, $|b| = b$:\n",
        "- Substitute:\n",
        "\\begin{gather}\n",
        "|a + b| = a + b = |a| + |b|\n",
        "\\end{gather}\n",
        "\n",
        "**In Conclusion**, the inequality is proven.\n",
        "\n",
        "<br><br>\n",
        "\n",
        "3. Prove the triangle inequality $|x+y| \\leq |x| + |y|, \\forall (x,y) \\in \\mathbb{R}$\n",
        "\n",
        "Step 1: Definition of an absolute value\n",
        "\n",
        "- Definition\n",
        "\\begin{gather}\n",
        "{|x| = }\n",
        "\\begin{cases}\n",
        "x,&{x \\geq 0}\\\\ -x,&{x < 0}\n",
        "\\end{cases}\n",
        "\\end{gather}\n",
        "\n",
        "- Thus, we must solve for 4 cases:\n",
        "\n",
        "\\begin{gather}\n",
        "\\text{Case 1: }{x \\geq 0, y \\geq 0} \\\\\n",
        "\\text{Case 2: }{x < 0, y < 0} \\\\\n",
        "\\text{Case 3: }{x \\geq 0, y < 0} \\\\\n",
        "\\text{Case 4: }{x < 0, y \\geq 0} \\\\\n",
        "\\end{gather}\n",
        "\n",
        "Case 1: $x \\geq 0, y \\geq 0$\n",
        "\n",
        "- Let, $|x + y| = x + y$, and $|x| = x, |y| = y$\n",
        "- Substitution:\n",
        "\\begin{gather}\n",
        "|x + y| = x + y = |x| + |y|\n",
        "\\end{gather}\n",
        "\n",
        "Case 2: $x < 0, y < 0$\n",
        "\n",
        "- Let, $|x + y| = -(x + y)$, and $|x| = -x, |y| = -y$\n",
        "- Substitution:\n",
        "\\begin{gather}\n",
        "|x + y| = -(x + y) = -x + (-y) = |x| + |y|\n",
        "\\end{gather}\n",
        "\n",
        "Case 3: $x \\geq 0, y < 0$\n",
        "\n",
        "- Let, $|x| = x, |y| = -y$\n",
        "- Substitution:\n",
        "\\begin{gather}\n",
        "|x + y| \\leq x - y\n",
        "\\end{gather}\n",
        "- Since, $x$  is non-negative and $y$ is negative, $x - y$ could be either positive or negative. So, let's consider both possibilities:\n",
        "\n",
        "For $x + y \\geq 0$:\n",
        "\\begin{gather}\n",
        "x + y \\leq x - y \\\\  \n",
        "y \\leq -y\n",
        "\\end{gather}\n",
        "\n",
        "For $x + y < 0$:\n",
        "\\begin{gather}\n",
        "-(x + y) \\leq x - y \\\\\n",
        "-x - y \\leq x - y \\\\\n",
        "-x \\leq x\n",
        "\\end{gather}}\n",
        "\n",
        "Case 4: $x < 0, y \\geq 0$\n",
        "\n",
        "- Let, $|x| = -x, |y| = y$\n",
        "- Substitution:\n",
        "\\begin{gather}\n",
        "|x + y| \\leq -x + y\n",
        "\\end{gather}\n",
        "- Solve for sub-cases of $|x + y|$:\n",
        "\\begin{gather}\n",
        "x + y, x + y \\geq 0 \\\\\n",
        "-(x + y), x + y < 0 \\\\\n",
        "\\end{gather}\n",
        "\n",
        "For $x + y \\geq 0$:\n",
        "\\begin{gather}\n",
        "x + y \\leq -x + y \\\\\n",
        "x \\leq -x\n",
        "\\end{gather}\n",
        "\n",
        "For $x + y < 0$:\n",
        "\\begin{gather}\n",
        "-(x + y) \\leq -x + y \\\\\n",
        "-x - y \\leq -x + y \\\\\n",
        "-y \\leq y\n",
        "\\end{gather}\n",
        "\n",
        "**In Conclusion**, in all cases, $|x+y| \\leq |x| + |y| \\in \\mathbb{R} $\n",
        "\n",
        "\n",
        "<br> <br>\n",
        "\n",
        "4. Prove Sedrakayan's Lemma $\\forall u_i, v_i \\in \\mathbb{R}^+$:\n",
        "\\begin{gather}\n",
        "\\frac{(\\Sigma_{i=1}^n u_i)^2}{\\Sigma_{i=1}^n v_i}\n",
        "\\leq\n",
        "\\Sigma_{i=1}^n \\frac{(u_i)^2}{v_i}\n",
        "\\end{gather}\n",
        "\n",
        "\n",
        "Step 1: To prove Sedrakayan’s Lemma directly, we need to show that for all $(u_i, v_i \\in \\mathbb{R}^+)$, the inequality\n",
        "\n",
        "$$\\left(\\frac{\\sum_{i=1}^n u_i}{\\sum_{i=1}^n v_i}\\right)^2 \\leq \\frac{\\sum_{i=1}^n (u_i)^2}{v_i}$$\n",
        "\n",
        "holds true.\n",
        "\n",
        "Step 2: The **Cauchy-Schwarz Inequality** states that for any real numbers $(a_i)$ and $(b_i)$,\n",
        "\n",
        "$$\\left(\\sum_{i=1}^n a_i b_i\\right)^2 \\leq \\left(\\sum_{i=1}^n (a_i)^2\\right) \\left(\\sum_{i=1}^n (b_i)^2\\right)$$\n",
        "\n",
        "Step 3: Let $a_i = \\sqrt{u_i}$ and $b_i = \\frac{1}{\\sqrt{v_i}}$. Then, the Cauchy-Schwarz Inequality becomes\n",
        "\n",
        "$$\\left(\\sum_{i=1}^n \\sqrt{u_i} \\cdot \\frac{1}{\\sqrt{v_i}}\\right)^2 \\leq \\left(\\sum_{i=1}^n u_i\\right) \\left(\\sum_{i=1}^n \\frac{1}{v_i}\\right)$$\n",
        "\n",
        "**SIMPLIFY:**\n",
        "\n",
        "Step 4: The *left-hand side* simplifies to\n",
        "\n",
        "$$\\left(\\frac{\\sum_{i=1}^n u_i}{\\sum_{i=1}^n v_i}\\right)^2$$\n",
        "\n",
        "Step 5: The *right-hand side* simplifies to\n",
        "\n",
        "$$\\frac{\\sum_{i=1}^n (u_i)^2}{v_i}$$\n",
        "\n",
        "**In Conclusion**, since the left-hand side is less than or equal to the right-hand side, we have proven Sedrakayan’s Lemma.\n"
      ],
      "metadata": {
        "id": "tx_w5JEYbNGy"
      }
    }
  ]
}